Spacetalk/Step.lean
@@ -35,7 +35,7 @@ inductive UnaryOp : Ty → Ty → Type
   | mulConst : {w : Nat} → BitVec w → UnaryOp (BitVecTy w) (BitVecTy w)
 
 inductive Prog : List Ty → Ty → Type
-  | const : {α : Ty} → Prog [α] α
+  | id : {α : Ty} → Prog [α] α
   | zip : BinaryOp α β γ → Prog aInp α → Prog bInp β → Prog (aInp ++ bInp) γ
   | map : UnaryOp α β → Prog inp α → Prog inp β
   | reduce : BinaryOp α β α → Nat → α.denote → Prog inp β → Prog inp α
@@ -51,7 +51,7 @@ def UnaryOp.denote : UnaryOp α β → α.denote → β.denote
   | UnaryOp.mulConst c => BitVec.mul c
 
 def Prog.denote {inputs : List Ty} {α : Ty} : Prog inputs α → (DenoStreamsList inputs → DenoStreamsList [α])
-  | .const => λ ([a]ₕ) ↦ [a]ₕ
+  | .id => λ ([a]ₕ) ↦ [a]ₕ
   | .zip op as bs => λ inp ↦ let (aInp, bInp) := inp.split; [Stream'.zip op.denote (as.denote aInp).head (bs.denote bInp).head]ₕ
   | .map op as => λ inp ↦ [Stream'.map op.denote (as.denote inp).head]ₕ
   | .reduce op n init bs => λ inp ↦ [Stream'.reduce op.denote n init (bs.denote inp).head]ₕ
@@ -60,8 +60,8 @@ def Prog.denote {inputs : List Ty} {α : Ty} : Prog inputs α → (DenoStreamsLi
 
 declare_syntax_cat step
 
-syntax "const_32" : step
-syntax "const_64" : step
+syntax "id_32" : step
+syntax "id_64" : step
 
 syntax:50 step:50 " +z " step:51 : step
 syntax:60 step:60 " *z " step:61 : step
@@ -74,8 +74,8 @@ syntax " ( "step " ) " : step
 syntax " 〚 " step " 〛 " : term
 
 macro_rules
-  | `(〚 const_32 〛) => `(@Prog.const (BitVecTy 32))
-  | `(〚 const_64 〛) => `(@Prog.const (BitVecTy 64))
+  | `(〚 id_32 〛) => `(@Prog.id (BitVecTy 32))
+  | `(〚 id_64 〛) => `(@Prog.id (BitVecTy 64))
   | `(〚 $a:step +z $b:step 〛) => `(Prog.zip .add 〚 $a 〛 〚 $b 〛)
   | `(〚 $a:step *z $b:step 〛) => `(Prog.zip .mul 〚 $a 〛 〚 $b 〛)
   | `(〚 $n:term +r start $init:term on ($a:step) 〛) => `(Prog.reduce .add $n $init 〚 $a 〛)
@@ -83,6 +83,6 @@ macro_rules
   | `(〚 ( $x ) 〛) => `(〚 $x 〛)
   | `(〚 $x 〛) => `(〚 $x 〛)
 
-#check 〚 const_32 +z (10 +r start 0 on ((const_32 +z const_32) *z const_32)) 〛
+#check 〚 id_32 +z (10 +r start 0 on ((id_32 +z id_32) *z id_32)) 〛
 
 end Step
